templates/flows/flows_big_op.v
@@ -1,3 +1,5 @@
+(* Big op over flows *)
+
 Set Default Proof Using "All".
 From iris.algebra Require Export big_op.
 Require Export flows ccm_big_op.
