templates/lockfree/skiplist_search.v
@@ -11,7 +11,7 @@ From iris.heap_lang.lib Require Import nondet_bool.
 From iris.bi.lib Require Import fractional.
 Set Default Proof Using "All".
 From iris.bi.lib Require Import fractional.
-(* Require Import skiplist_util. *)
+Require Import array_util.
 Require Export traverse_spec_module flows.
 
 
@@ -20,21 +20,21 @@ Module Type SKIPLIST_SEARCH.
   Export TR_SPEC TR_SPEC.SK_UTIL TR_SPEC.SK_UTIL.SK TR_SPEC.SK_UTIL.DEFS.
   Export TR_SPEC.SK_UTIL.SK.TR TR_SPEC.SK_UTIL.SK.TR.NODE.
 
-  Lemma searchOp_spec Σ Hg1 Hg2 Hg3 N γ_t γ_r γ_m γ_mt γ_msy r (p: proph_id) 
+  Lemma searchOp_spec Σ Hg1 Hg2 Hg3 N γ_t γ_r γ_m γ_mt γ_msy r (pr: proph_id) 
     pvs tid t0 Q k (hd tl: Node) :
       main_inv Σ Hg1 Hg2 Hg3 N γ_t γ_r γ_m γ_mt γ_msy r -∗
       thread_start Σ Hg1 Hg2 Hg3 γ_t γ_mt tid t0 -∗
       □ update_helping_protocol Σ Hg1 Hg2 Hg3 N γ_t γ_r γ_mt γ_msy -∗
       ⌜local_pre (searchOp k)⌝ -∗
       r ↦□ (#hd, #tl) -∗
-        {{{ proph p pvs ∗ 
+        {{{ proph pr pvs ∗ 
             (match process_proph tid pvs with
               contra => au Σ Hg1 Hg2 Hg3 N γ_r (searchOp k) Q
             | no_upd => True
             | upd => au Σ Hg1 Hg2 Hg3 N γ_r (searchOp k) Q end) }}}
               search #hd #tl #k @ ⊤
         {{{ (res: resT) prf pvs', RET #res;
-            proph p pvs' ∗ ⌜pvs = prf ++ pvs'⌝ ∗
+            proph pr pvs' ∗ ⌜pvs = prf ++ pvs'⌝ ∗
             (match process_proph tid pvs with
               contra => ⌜Forall (λ x, x.2 ≠ #tid) prf⌝
             | no_upd => past_lin_witness Σ Hg1 Hg2 Hg3 γ_m (searchOp k) res t0
@@ -43,10 +43,14 @@ Module Type SKIPLIST_SEARCH.
   Proof. 
     iIntros "#HInv #Thd_st #Upd [%HL %Range_k] #HR'". 
     iIntros (Φ) "!# (Hproph & Hmatch) Hpost".
-    wp_lam. wp_pures.
-    wp_apply traverse_spec; try done.
-    iIntros (preds succs ps ss res) "(Hpreds & Hsuccs & %Len_ps 
-      & %Len_ss & %HpsL & %HssL & #Htr)".  
+    wp_lam. wp_pures. wp_bind (AllocN _ _)%E. iApply array_repeat. iPureIntro; lia.
+    iNext. iIntros (preds) "Hpreds". wp_pures. wp_bind (AllocN _ _)%E.
+    iApply array_repeat. iPureIntro; lia. iNext. iIntros (succs) "Hsuccs". wp_pures.
+    wp_apply (traverse_spec Σ Hg1 Hg2 Hg3 with "[] [] [] [] [] [Hpreds Hsuccs]"); try done.
+    { iFrame "∗". iPureIntro. rewrite !replicate_length. rewrite !lookup_total_replicate_2.
+      done. all : lia. }
+    iIntros (p c ps ss res) "(Hpreds & Hsuccs & %Len_ps & %Len_ss & %HpsL & %HssL 
+      & %Hps0 & %Hss0 & #Htr)".
     wp_pures. 
     iInv "HInv" as (M0 T0 s0) "(>Ds & >%Habs0 & >Hist & Help & >Templ)".
     iDestruct "Templ" as (hd' tl' γ_ks)"(HR & SShot0 & Res & %PT0 & %Trans_M0)".
@@ -55,7 +59,6 @@ Module Type SKIPLIST_SEARCH.
     iAssert (past_lin_witness _ _ _ _ γ_m (searchOp k) res t0)%I as "#PastW".
     { iDestruct "Htr" as "(_ & Htr)". 
       iDestruct "Htr" as (s)"(#Past_s & %H')". 
-      set c := ss !!! 0. rewrite -/c in H'.
       iPoseProof (per_tick_past with "[%] Hist Past_s") as "%PT_s"; try done.
       iExists s. iFrame "#". iPureIntro. rewrite /seq_spec. split. done.
       destruct H' as (H' & H'' & H'''). destruct PT_s as (_&_&PT&_).
