templates/lockfree/traverse_spec_module.v
@@ -9,6 +9,8 @@ From iris.bi.lib Require Import fractional.
 From flows Require Import array_util skiplist_util.
 Set Default Proof Using "All".
 
+(* Traversal Spec *)
+
 Module Type TRAVERSE_SPEC.
   Declare Module SK_UTIL : SKIPLIST_UTIL.
   Export SK_UTIL SK_UTIL.DEFS SK_UTIL.DEFS.DS.
@@ -18,105 +20,26 @@ Module Type TRAVERSE_SPEC.
     (∃ s, past_state Σ Hg1 Hg2 Hg3 γ_m t0 s 
         ∗ ⌜p ∈ FP s ∧ i < Height s p ∧ Key s p < k⌝)
   ∗ (∃ s, past_state Σ Hg1 Hg2 Hg3 γ_m t0 s ∗ ⌜c ∈ FP s ∧ i < Height s c⌝).
-
-  Lemma traversal_inv_hd_tl Σ Hg1 Hg2 Hg3 γ_m γ_t γ_mt hd tl M T s tid t0 k:
-    ⌜M !!! T ≡ s⌝ -∗ 
-    ⌜per_tick_inv hd tl s⌝ -∗
-    ⌜1 < L⌝ -∗
-    ⌜0 < k < W⌝ -∗
-    thread_start Σ Hg1 Hg2 Hg3 γ_t γ_mt tid t0 -∗
-    hist Σ Hg1 Hg2 Hg3 γ_t γ_m M T -∗
-      |==> traversal_inv Σ Hg1 Hg2 Hg3 γ_m t0 (L-1) k hd tl ∗ hist Σ Hg1 Hg2 Hg3 γ_t γ_m M T.
-  Proof.
-    iIntros "%Habs %PT %HL %Range_k #Thd_st Hist".
-    iPoseProof (snapshot_current with "[%] [#] [$]") 
-      as ">(#Past_s&Hist)"; try done.
-    destruct PT as ((H1'&H2'&H3'&H4'&H5'&H6'&H7'&H8'&H9')&_).
-    iModIntro. iFrame. iSplit; iExists s; iFrame "Past_s".
-    - iPureIntro; repeat split; try (done || lia).
-      set_solver.
-    - iPureIntro; repeat split; try (done || lia). set_solver.
-  Qed. 
-
-  Parameter traverse_rec_spec : ∀ Σ Hg1 Hg2 Hg3 N γ_t γ_r γ_m γ_mt γ_msy r tid 
-    t0 k preds succs ps0 ss0 (i: nat) (hd tl: Node),
+  
+  Parameter traverse_spec : ∀ Σ Hg1 Hg2 Hg3 N γ_t γ_r γ_m γ_mt γ_msy r tid t0 k (hd tl: Node)
+    preds succs ps0 ss0,
     main_inv Σ Hg1 Hg2 Hg3 N γ_t γ_r γ_m γ_mt γ_msy r -∗
     thread_start Σ Hg1 Hg2 Hg3 γ_t γ_mt tid t0 -∗
     □ update_helping_protocol Σ Hg1 Hg2 Hg3 N γ_t γ_r γ_mt γ_msy -∗ 
     ⌜1 < L ∧ 0 < k < W⌝ -∗
     r ↦□ (#hd, #tl) -∗
       {{{ is_array Σ Hg1 preds ps0 ∗ is_array Σ Hg1 succs ss0
-          ∗ ⌜length ps0 = L⌝ ∗ ⌜length ss0 = L⌝ ∗ ⌜i+1 < L⌝
-          ∗ ⌜ps0 !!! (L-1) = hd⌝ ∗ ⌜ss0 !!! (L-1) = tl⌝
-          ∗ (∀ j, ⌜i < j < L⌝ → 
-              traversal_inv Σ Hg1 Hg2 Hg3 γ_m t0 j k (ps0 !!! j) (ss0 !!! j)
-            ∗ (∃ s, past_state Σ Hg1 Hg2 Hg3 γ_m t0 s 
-                        ∗ ⌜(ps0 !!! j) ∈ FP s ∧ Marki s (ps0 !!! j) 0 = false⌝)) }}}
-        traverse_rec #k #preds #succs #i @ ⊤
-      {{{ (ps ss: list Node) (res: bool), 
-            RET (#preds, #succs, #res);
+          ∗ ⌜length ps0 = L⌝ ∗ ⌜length ss0 = L⌝
+          ∗ ⌜ps0 !!! (L-1) = hd⌝ ∗ ⌜ss0 !!! (L-1) = tl⌝ }}}
+          traverse #hd #tl #preds #succs #k @ ⊤
+      {{{ (p c : Node) (ps ss: list Node) (res: bool), 
+            RET (#p, #c, #res);
             is_array Σ Hg1 preds ps ∗ is_array Σ Hg1 succs ss
           ∗ ⌜length ps = L⌝ ∗ ⌜length ss = L⌝
           ∗ ⌜ps !!! (L-1) = hd⌝ ∗ ⌜ss !!! (L-1) = tl⌝
+          ∗ ⌜ps !!! 0 = p⌝ ∗ ⌜ss !!! 0 = c⌝
           ∗ (∀ i, ⌜i < L⌝ → traversal_inv Σ Hg1 Hg2 Hg3 γ_m t0 i k (ps !!! i) (ss !!! i))
-          ∗ (let c := ss !!! 0 in 
-              ∃ s, past_state Σ Hg1 Hg2 Hg3 γ_m t0 s ∗
-                ⌜c ∈ FP s ∧ k ∈ keyset (FI s c) ∧ (res ↔ k ∈ Content s c)⌝) }}}.
-
-  
-  Lemma traverse_spec Σ Hg1 Hg2 Hg3 N γ_t γ_r γ_m γ_mt γ_msy r tid t0 k (hd tl: Node):
-    main_inv Σ Hg1 Hg2 Hg3 N γ_t γ_r γ_m γ_mt γ_msy r -∗
-    thread_start Σ Hg1 Hg2 Hg3 γ_t γ_mt tid t0 -∗
-    □ update_helping_protocol Σ Hg1 Hg2 Hg3 N γ_t γ_r γ_mt γ_msy -∗ 
-    ⌜1 < L ∧ 0 < k < W⌝ -∗
-    r ↦□ (#hd, #tl) -∗
-      {{{ True }}}
-          traverse #hd #tl #k @ ⊤
-      {{{ (preds succs: loc) (ps ss: list Node) (res: bool), 
-            RET (#preds, #succs, #res);
-            (preds ↦∗ ((fun n => # (LitLoc n)) <$> ps))
-          ∗ (succs ↦∗ ((fun n => # (LitLoc n)) <$> ss))
-          ∗ ⌜length ps = L⌝ ∗ ⌜length ss = L⌝
-          ∗ ⌜ps !!! (L-1) = hd⌝ ∗ ⌜ss !!! (L-1) = tl⌝
-          ∗ (∀ i, ⌜i < L⌝ → traversal_inv Σ Hg1 Hg2 Hg3 γ_m t0 i k (ps !!! i) (ss !!! i))
-          ∗ (let c := ss !!! 0 in 
-                ∃ s, past_state Σ Hg1 Hg2 Hg3 γ_m t0 s ∗
+          ∗ (∃ s, past_state Σ Hg1 Hg2 Hg3 γ_m t0 s ∗
                     ⌜c ∈ FP s ∧ k ∈ keyset (FI s c) ∧ (res ↔ k ∈ Content s c)⌝) }}}.
-  Proof.
-    iIntros "#HInv #Thd_st #Upd [%HL %Range_k] #HR'". iIntros (Φ) "!# _ Hpost".
-    wp_lam. wp_pures. wp_bind (AllocN _ _)%E. 
-    iApply array_repeat. iPureIntro; lia.
-    iNext. iIntros (preds) "Hpreds".
-    wp_pures. wp_bind (AllocN _ _)%E.
-    iApply array_repeat. iPureIntro; lia.
-    iNext. iIntros (succs) "Hsuccs". wp_pures. iApply fupd_wp.
-    iInv "HInv" as (M0 T0 s0) "(>Ds & >%Habs0 & >Hist & Help & >Templ)".
-    iDestruct "Templ" as (hd' tl' γ_ks)"(HR & SShot0 & Res & %PT0 & %Trans_M0)".
-    iAssert (⌜hd' = hd ∧ tl' = tl⌝)%I with "[HR]" as %[-> ->]. 
-    { iDestruct (mapsto_agree with "[$HR] [$HR']") as %[=]. by iPureIntro. }
-    iAssert (⌜per_tick_inv hd tl s0⌝)%I as %PT_s0.
-    { iApply (per_tick_current with "[%] [%] [$Hist]"); try done. }
-    iPoseProof (traversal_inv_hd_tl with "[%] [%] [%] [%] [#] [Hist]") 
-      as ">(#HtrL & Hist)"; try done.
-    iPoseProof (snapshot_current with "[%] [#] [$Hist]") 
-      as ">(#Past_s0&Hist)"; try done.
-    iAssert (∃ s, past_state Σ Hg1 Hg2 Hg3 γ_m t0 s ∗
-      ⌜hd ∈ FP s ∧ Marki s hd 0 = false⌝)%I as "Marked_hd".
-    { iExists s0. iFrame "Past_s0". iPureIntro. destruct PT_s0 as (PT&_).
-      destruct PT as (H'&_&_&H''&_). split. set_solver. apply H''. lia. }
-    iModIntro. iSplitR "Hpreds Hsuccs Hpost".
-    { iNext. iExists M0, T0, s0. iFrame "∗%". iExists hd, tl, γ_ks. iFrame "∗%". }
-    iModIntro.    
-    wp_apply (traverse_rec_spec with "[] [] [] [] [] [Hpreds Hsuccs]"); try done.
-    iFrame "Hpreds Hsuccs".
-    iSplitR. iPureIntro. by rewrite replicate_length.
-    iSplitR. iPureIntro. by rewrite replicate_length.
-    iSplitR. iPureIntro. clear -HL; lia.
-    iSplitR. iPureIntro. rewrite lookup_total_replicate_2. done. lia.
-    iSplitR. iPureIntro. rewrite lookup_total_replicate_2. done. lia.
-    iIntros (j) "%Hj". 
-    assert (j = L-1) as -> by lia. rewrite !lookup_total_replicate_2.
-    all : try lia. iFrame "HtrL Marked_hd".
-  Qed.
 
 End TRAVERSE_SPEC.
