templates/util/gset_seq.v
@@ -1,30 +1,96 @@
 From stdpp Require Import list.
 From iris.algebra Require Import gset numbers.
+From flows Require Import flows.
 
-Definition gset_seq i j : gset nat :=
-  list_to_set (seq i (j + 1 - i)).
+  (* Define gset representing [n1 ... n2]; and its properties *)
 
-Lemma elem_of_gset_seq i j k :
-  k ∈ gset_seq i j ↔ i ≤ k ≤ j.
-Proof.
-  intros; rewrite elem_of_list_to_set elem_of_seq; lia.
-Qed.
+  Definition gset_seq i j : gset nat :=
+    list_to_set (seq i (j + 1 - i)).
 
-Lemma gset_seq_eq T T' :
-  gset_seq 0 T = gset_seq 0 T' → T = T'.
-Proof.
-  intros Heq. 
-  assert (T ∈ gset_seq 0 T') as HT. 
-  { rewrite -Heq elem_of_gset_seq. lia. }
-  assert (T' ∈ gset_seq 0 T) as HT'. 
-  { rewrite Heq elem_of_gset_seq. lia. }
-  rewrite !elem_of_gset_seq in HT HT'. lia.
-Qed.
+  Lemma elem_of_gset_seq i j k :
+    k ∈ gset_seq i j ↔ i ≤ k ≤ j.
+  Proof.
+    intros; rewrite elem_of_list_to_set elem_of_seq; lia.
+  Qed.
 
-Lemma gset_seq_union T :
-gset_seq 0 (T+1) = gset_seq 0 T ∪ {[T+1]}.
-Proof.
-  apply set_eq_subseteq. split.
-  all: intros x; rewrite elem_of_union !elem_of_gset_seq elem_of_singleton; lia.
-Qed.
+  Lemma gset_seq_eq T T' :
+    gset_seq 0 T = gset_seq 0 T' → T = T'.
+  Proof.
+    intros Heq. 
+    assert (T ∈ gset_seq 0 T') as HT. 
+    { rewrite -Heq elem_of_gset_seq. lia. }
+    assert (T' ∈ gset_seq 0 T) as HT'. 
+    { rewrite Heq elem_of_gset_seq. lia. }
+    rewrite !elem_of_gset_seq in HT HT'. lia.
+  Qed.
 
+  Lemma gset_seq_union T :
+  gset_seq 0 (T+1) = gset_seq 0 T ∪ {[T+1]}.
+  Proof.
+    apply set_eq_subseteq. split.
+    all: intros x; rewrite elem_of_union !elem_of_gset_seq elem_of_singleton; lia.
+  Qed.
+
+  Lemma mark_map (h: nat) :
+    h > 0 →
+      ∃ (m: gmap nat bool), (∀ i, i < h → m !! i = Some false) 
+        ∧ dom m = gset_seq 0 (h-1).
+  Proof.
+    intros Hz.
+    Fixpoint f n (res: gmap nat bool) := 
+      match n with S n' => f n' (<[n' := false]> res) | 0 => res end.
+    set m := f h ∅.
+    assert (∀ n res i, (i < n → f n res !! i = Some false) ∧ 
+                  (¬ i < n → f n res !! i = res !! i)) as H'.
+    { clear. induction n.
+      - intros res i; split; first by lia. intros H'; by simpl.
+      - intros res i. pose proof IHn (<[n:=false]> res) i as H''.
+        split; intros Hi; simpl.
+        + destruct (decide (i = n)) as [-> | Hin].
+          { assert (¬ n < n) as H' by lia. 
+            destruct H'' as [_ H'']. pose proof H'' H' as H''.
+            rewrite H'' lookup_insert. done. }
+          assert (i < n) as H'%H'' by lia. by rewrite H'.
+        + assert (¬ i < n) as H'%H'' by lia. rewrite H'.
+          rewrite lookup_insert_ne; try (done || lia). }
+    exists m. split. apply H'. pose proof H' h ∅ as H'. 
+    rewrite -/m in H'. apply set_eq_subseteq. split.
+    intros j Hj. destruct (decide (j < h)) as [Hj' | Hj']. 
+    rewrite elem_of_gset_seq. lia. apply H' in Hj'. 
+    rewrite lookup_empty -not_elem_of_dom in Hj'. done.
+    intros j Hj. rewrite elem_of_gset_seq in Hj. 
+    assert (j < h) as H'' by lia. apply H' in H''.
+    rewrite elem_of_dom H''. done.    
+  Qed.
+
+  Lemma next_map (h: nat) (ss : list Node) :
+    h > 0 →  
+      (∃ (nx: gmap nat Node), (∀ i, i < h → nx !! i = Some (ss !!! i))
+        ∧ dom nx = gset_seq 0 (h-1)).
+  Proof.
+    intros Hz.
+    Fixpoint f' (l: list Node) n (res: gmap nat Node) := 
+        match n with S n' => f' l n' (<[n':= l !!! n']> res) | 0 => res end.
+      set nx := f' ss h ∅.
+      assert (∀ n res i, (i < n → f' ss n res !! i = Some (ss !!! i)) ∧ 
+                    (¬ i < n → f' ss n res !! i = res !! i)) as H'.
+      { clear. induction n.
+        - intros res i; split; first by lia. intros H'; by simpl.
+        - intros res i. pose proof IHn (<[n:=(ss !!! n)]> res) i as H''.
+          split; intros Hi; simpl.
+          + destruct (decide (i = n)) as [-> | Hin].
+            { assert (¬ n < n) as H' by lia. 
+              destruct H'' as [_ H'']. pose proof H'' H' as H''.
+              rewrite H'' lookup_insert. done. }
+            assert (i < n) as H'%H'' by lia. by rewrite H'.
+          + assert (¬ i < n) as H'%H'' by lia. rewrite H'.
+            rewrite lookup_insert_ne; try (done || lia). }
+      exists nx. split. apply H'. pose proof H' h ∅ as H'. 
+      rewrite -/nx in H'. apply set_eq_subseteq. split.
+      intros j Hj. destruct (decide (j < h)) as [Hj' | Hj']. 
+      rewrite elem_of_gset_seq. lia. apply H' in Hj'. 
+      rewrite lookup_empty -not_elem_of_dom in Hj'. done.
+      intros j Hj. rewrite elem_of_gset_seq in Hj. 
+      assert (j < h) as H'' by lia. apply H' in H''.
+      rewrite elem_of_dom H''. done.
+  Qed.
