templates/util/keyset_ra.v
@@ -3,6 +3,8 @@ From iris.proofmode Require Import tactics.
 From iris.base_logic.lib Require Export iprop.
 From iris.base_logic.lib Require Export invariants.
 
+(* Keyset RA *)
+
 Set Default Proof Using "All".
 (* Require Export search_str flows auth_ext.*)
 
